module TRS.TRS-Examples where

open import Logic
open import TRS.TRS-Base
open import Data.Fin
open import Data.Vec
open import Agda.Builtin.Nat renaming (Nat to â„•)
open import Classical
open import Relation.Nullary
open import Relations.ClosureOperators
open import Predicates
open import ARS.Properties

fdecFin : âˆ€ {n : â„•} â†’ (x y : Fin n) â†’ EM (x â‰¡ y)
fdecFin x y with x â‰Ÿ y
... | yes p = in1 p
... | no Â¬p = in2 (Î» x=y â†’ âŠ¥-elim (Â¬p x=y)) where open import Data.Empty using (âŠ¥-elim)

module Example1 where
  -- p1: F(a,x) -> G(x,x)
  -- p2: b -> F(b,b)
  -- Taken from Example 2.2.8 in TeReSe

  S : Signature
  S = Sig (Fin 4) ar (Î» {x} {y} â†’ fdecFin x y )  where
    ar : _
    ar zero = 0 -- a
    ar (suc zero) = 0 -- b
    ar (suc (suc zero)) = 2 -- F
    ar (suc (suc (suc zero))) = 2 -- G
 

  open Signature S
  open Substitution S

  p1lhs : Pattern 1 -- F(a,x)
  p1lhs = funp (suc (suc zero)) (Pa âˆ· Px âˆ· []) where
    Pa = 0 ,, funp zero []
    Px = 1 ,, hole

  p2lhs : Pattern 0 -- b
  p2lhs = funp (suc zero) []

  p1 : RRule
  p1 = RR 1 p1lhs (fun (suc (suc (suc zero))) (var zero âˆ· var zero âˆ· []) )

  p2 : RRule
  p2 = RR 0 p2lhs (fun (suc (suc zero)) (b âˆ· b âˆ· []) )
    where b = fun (suc zero) []

  p12 : Fin 2 â†’ RRule 
  p12 zero = p1
  p12 (suc zero) = p2

  R12 : âˆ€ {V} â†’ ğ“¡ (Terms V)
  R12 {V} = GeneralTRS.InScope.R {RuleIdx = Fin 2} p12 V

  s : Terms âŠ¥  -- F(a,b)
  s = fun (suc (suc zero)) (fun zero [] âˆ· fun (suc zero) [] âˆ· [])

  t : Terms âŠ¥ -- G(b,F(b,b))
  t = fun (suc (suc (suc zero)))
        (fun (suc zero) []
        âˆ· fun (suc (suc zero)) (fun (suc zero) [] âˆ· fun (suc zero) [] âˆ· [])
        âˆ· [])

  sâ†’*t : (R12 â‹†) s t
  sâ†’*t = Rax (zero ,, refl)
      ,â‹† (Rfun (suc (suc (suc zero))) (b âˆ· b âˆ· []) (suc zero) bâ†’fbb refl refl ,â‹† Îµâ‹†)
    where
      b : Terms âŠ¥
      b = fun (suc zero) []

      fbb : Terms âŠ¥
      fbb = fun (suc (suc zero)) (b âˆ· b âˆ· [])

      bâ†’fbb : R12 b fbb
      bâ†’fbb = Rax ((suc zero) ,, refl)



module Example-aa where
    -- a -> a 
  -- Signature with one constant symbol a : 0-ary function
  S : Signature
  S = Sig (Fin 1) ar (Î» {x} {y} â†’ fdecFin x y ) where
    ar : Fin 1 â†’ â„• 
    ar zero = 0 -- a 


  open Signature S
  open Substitution S

  lhs-aa : Pattern  0 -- a 
  lhs-aa = funp zero []

  rhs-aa : Terms (Fin 0)
  rhs-aa = fun zero []

  rule-aa : RRule 
  rule-aa = RR 0 lhs-aa rhs-aa

  rules-aa : Fin 1 â†’ RRule 
  rules-aa zero = rule-aa

  Raa : âˆ€ {V} â†’ ğ“¡ (Terms V)
  Raa {V} = GeneralTRS.InScope.R  {RuleIdx = Fin 1} rules-aa V

  RaaâŠ¥ : ğ“¡ (Terms âŠ¥)
  RaaâŠ¥ = Raa {V = âŠ¥}
  -- showing this example is locally SM
  open LocalProperties {A = Terms âŠ¥} {R = RaaâŠ¥}

  a : Terms âŠ¥
  a = fun zero []

  aâ†’a : Raa a a
  aâ†’a = Rax (zero ,, refl)

  a-step-id : âˆ€ {y} â†’ RaaâŠ¥ a y â†’ y â‰¡ a
  a-step-id (Rax (zero ,, refl)) = refl
  a-step-id (Rfun .zero .[] () r refl refl)

  aâ†’*a-id : âˆ€ {y} â†’ (RaaâŠ¥ â‹†) a y â†’ y â‰¡ a
  aâ†’*a-id Îµâ‹† = refl
  aâ†’*a-id (Rxy ,â‹† R*xy) rewrite a-step-id Rxy = aâ†’*a-id R*xy

  aâˆˆMF : MF a
  aâˆˆMF y R*ay rewrite aâ†’*a-id R*ay = Îµâ‹†

  aâˆˆSM : SM a
  aâˆˆSM = MFâŠ†SM a aâˆˆMF

module Example-bubble where
  -- bubble-sort style swap:
  -- cons(x, cons(y, z)) -> cons(y, cons(x, z))

  S : Signature
  S = Sig (Fin 1) ar (Î» {x} {y} â†’ fdecFin x y) where
    ar : Fin 1 â†’ â„•
    ar zero = 2 -- cons

  open Signature S
  open Substitution S

  lhs-swap : Pattern 3 -- cons(x, cons(y, z))
  lhs-swap = funp zero (Px âˆ· Pyz âˆ· []) where
    Px : Î£-syntax â„• Pattern
    Px = 1 ,, hole

    Py : Î£-syntax â„• Pattern
    Py = 1 ,, hole

    Pz : Î£-syntax â„• Pattern
    Pz = 1 ,, hole

    Pyz : Î£-syntax â„• Pattern
    Pyz = 2 ,, funp zero (Py âˆ· Pz âˆ· [])
  
  rhs-swap : Terms (Fin 3) -- cons(y, cons(x, z))
  rhs-swap = fun zero
    (var (suc zero) âˆ· fun zero (var zero âˆ· var (suc (suc zero)) âˆ· []) âˆ· [])

  rule-swap : RRule
  rule-swap = RR 3 lhs-swap rhs-swap

  rules-swap : Fin 1 â†’ RRule
  rules-swap zero = rule-swap

  Rswap : âˆ€ {V} â†’ ğ“¡ (Terms V)
  Rswap {V} = GeneralTRS.InScope.R {RuleIdx = Fin 1} rules-swap V

  tâ‚ : Terms (Fin 3)
  tâ‚ = fun zero (var zero âˆ· fun zero (var (suc zero) âˆ· var (suc (suc zero)) âˆ· []) âˆ· [])

  tâ‚‚ : Terms (Fin 3)
  tâ‚‚ = fun zero (var (suc zero) âˆ· fun zero (var zero âˆ· var (suc (suc zero)) âˆ· []) âˆ· [])

  tâ‚â†’tâ‚‚ : Rswap tâ‚ tâ‚‚
  tâ‚â†’tâ‚‚ = Rax (zero ,, refl)

module Example-NewmanCandidate where

  -- aS : Fin 5
  -- aS = zero
  --
  -- bS : Fin 5
  -- bS = suc zero
  --
  -- pS : Fin 5
  -- pS = suc (suc zero)
  --
  -- fS : Fin 5
  -- fS = suc (suc (suc zero))
  --
  -- kS : Fin 5
  -- kS = suc (suc (suc (suc zero)))

  pattern aS = zero 
  pattern bS = suc zero 
  pattern pS = suc (suc zero) 
  pattern fS = suc (suc (suc zero)) 
  pattern kS = suc (suc (suc (suc zero)))


  -- Rules:
  --   p(a) -> p(b)
  --   p(b) -> p(a)
  --   f(p(a), p(a)) -> k
  --   f(p(b), p(b)) -> k

  S : Signature
  S = Sig (Fin 5) ar (Î» {x} {y} â†’ fdecFin x y) where
    ar : Fin 5 â†’ â„•
    ar aS = 0 -- a
    ar bS = 0 -- b
    ar pS = 1 -- p
    ar fS = 2 -- f
    ar kS = 0 -- k

  open Signature S
  open Substitution S

  lhsâ‚ : Pattern 0
  lhsâ‚ = funp pS ((0 ,, funp aS []) âˆ· [])

  rhsâ‚ : Terms (Fin 0)
  rhsâ‚ = funpâ†’term where
    funpâ†’term : Terms (Fin 0)
    funpâ†’term = fun pS (fun bS [] âˆ· [])

  lhsâ‚‚ : Pattern 0
  lhsâ‚‚ = funp pS ((0 ,, funp bS []) âˆ· [])

  rhsâ‚‚ : Terms (Fin 0)
  rhsâ‚‚ = fun pS (fun aS [] âˆ· [])

  lhsâ‚ƒ : Pattern 0
  lhsâ‚ƒ = funp fS ((0 ,, funp pS ((0 ,, funp aS []) âˆ· []))
               âˆ· (0 ,, funp pS ((0 ,, funp aS []) âˆ· []))
               âˆ· [])

  rhsâ‚ƒ : Terms (Fin 0)
  rhsâ‚ƒ = fun kS []

  lhsâ‚„ : Pattern 0
  lhsâ‚„ = funp fS ((0 ,, funp pS ((0 ,, funp bS []) âˆ· []))
               âˆ· (0 ,, funp pS ((0 ,, funp bS []) âˆ· []))
               âˆ· [])

  rhsâ‚„ : Terms (Fin 0)
  rhsâ‚„ = fun kS []

  râ‚ : RRule
  râ‚ = RR 0 lhsâ‚ rhsâ‚

  râ‚‚ : RRule
  râ‚‚ = RR 0 lhsâ‚‚ rhsâ‚‚

  râ‚ƒ : RRule
  râ‚ƒ = RR 0 lhsâ‚ƒ rhsâ‚ƒ

  râ‚„ : RRule
  râ‚„ = RR 0 lhsâ‚„ rhsâ‚„

  rules : Fin 4 â†’ RRule
  rules zero = râ‚
  rules (suc zero) = râ‚‚
  rules (suc (suc zero)) = râ‚ƒ
  rules (suc (suc (suc zero))) = râ‚„

  Rnc : âˆ€ {V} â†’ ğ“¡ (Terms V)
  Rnc {V} = GeneralTRS.InScope.R {RuleIdx = Fin 4} rules V

  open LocalProperties
  -- open Substitution

  -- open Signature 
  {- Plan: 
  -- a,b,k are normal forms 
  -- p(a), p(b) are minimal forms 
  -- the rhs of each rule results in one of the above
  -- f(p(a),p(b)) -> f(p(a),p(a)) -> k 
  -- For p, need lemma: t ->â‹† a, then t = a, also if t ->â‹† b, then t = b
  --
  -- Needed lemmas:
  -- p(p(t)) ->â‹† p(u) â‡’ p(t) â†’ u 
  -- p(f(t1,t2)) ->â‹† p(u) â‡’ f(t1,t2) â†’ u
  -}

  -- p(p(t)) -> p(u) â‡’ p(t) â†’ u 
  -- p-lemma-1 : âˆ€ {V} (t : Terms V) (u : Terms V) 
  --               â†’ Rnc (fun pS (fun pS (t âˆ· []) âˆ· [])) (fun pS (u âˆ· []))
  --               â†’ Rnc (fun pS (t âˆ· [])) u
  -- p-lemma-1 t u (Substitution.Rax (suc (suc (suc zero)) ,, ()))
  -- p-lemma-1 t u (Substitution.Rax (suc (suc (suc (suc ()))) ,, sndâ‚))
  -- p-lemma-1 t u (Substitution.Rfun f ts zero Rtu refl refl) = Rtu

  p-lemma-1 : âˆ€ {V} (t : Terms V) (u : Terms V) 
                â†’ Rnc (fun pS (fun pS (t âˆ· []) âˆ· [])) u 
                â†’ Î£[ v âˆˆ Terms V ] ((u â‰¡ fun pS (v âˆ· [])) Ã— Rnc (fun pS (t âˆ· [])) v)
  p-lemma-1 t u (Substitution.Rax (suc (suc (suc zero)) ,, ()))
  p-lemma-1 t u (Substitution.Rax (suc (suc (suc (suc ()))) ,, sndâ‚))
  p-lemma-1 t u (Substitution.Rfun (suc (suc zero)) (v âˆ· []) zero {u = w} pptâ†’u refl refl) 
    = w ,, refl , pptâ†’u

  -- Base case easy. Induction step should be mix p-lemma1 with inductive call.
  p-lemma-1* : âˆ€ {V} (t : Terms V) (u : Terms V) 
                â†’ (Rnc â‹†) (fun pS (fun pS (t âˆ· []) âˆ· [])) u 
                â†’ Î£[ v âˆˆ Terms V ] ((u â‰¡ fun pS (v âˆ· [])) Ã— (Rnc â‹†) (fun pS (t âˆ· [])) v)
  
  -- p-lemma-1* t .(fun pS (fun pS (t âˆ· []) âˆ· [])) Îµâ‹† = fun pS (t âˆ· []) ,, refl , Îµâ‹† 
  -- p-lemma-1* t u (Rppty ,â‹† R*yu) with p-lemma-1 t _ Rppty 
  -- ... | v ,, refl , ptâ†’v = fun pS (v âˆ· []) ,, {! refl ,, ?  !} 
  p-lemma-1* t u Îµâ‹† = fun pS (t âˆ· []) ,, refl , Îµâ‹†
  p-lemma-1* t u (Substitution.Rax (fS ,, ()) ,â‹† Q)
  p-lemma-1* t u (Substitution.Rax (suc (suc (suc (suc ()))) ,, sndâ‚) ,â‹† R*yu)
  p-lemma-1* t u (Substitution.Rfun .pS .(fun pS (t âˆ· []) âˆ· []) aS (Substitution.Rax (aS ,, ar)) refl refl ,â‹† R*yu) with applyRuleInv rules _ _ _ _ ar 
  ...| sub ,, eq rewrite eq = {!   !}
  p-lemma-1* t u (Substitution.Rfun .pS .(fun pS (t âˆ· []) âˆ· []) j (Substitution.Rax (suc fstâ‚ ,, sndâ‚)) refl refl ,â‹† R*yu) = {!   !}
  p-lemma-1* t u (Substitution.Rfun f ts j (Substitution.Rfun fâ‚ tsâ‚ jâ‚ x xâ‚ƒ xâ‚„) xâ‚ xâ‚‚ ,â‹† R*yu) = {!   !} 
  --  with p-lemma-1 t u {!  x !} 
  -- ... | Q = {!   !} 

  -- p(f(t1,t2)) -> p(u) â‡’ f(t1,t2) â†’ u
  p-lemma-2 : âˆ€ {V} (t1 t2 u : Terms V)
                â†’ Rnc (fun pS (fun fS (t1 âˆ· t2 âˆ· []) âˆ· [])) u 
                â†’ Î£[ v âˆˆ Terms V ] ((u â‰¡ fun pS (v âˆ· [])) Ã— (Rnc (fun fS (t1 âˆ· t2 âˆ· [])) v))
  p-lemma-2 t1 t2 u (Substitution.Rax (suc (suc (suc zero)) ,, ()))
  p-lemma-2 t1 t2 u (Substitution.Rax (suc (suc (suc (suc ()))) ,, sndâ‚))
  p-lemma-2 t1 t2 u (Substitution.Rfun f ts zero {u = w} Rtu refl refl) = w ,, refl , Rtu

  p-lemma-3 :  âˆ€ {V} (t : Terms V) â†’ t âˆˆ MF {R = Rnc} â†’ fun pS (t âˆ· []) âˆˆ MF {R = Rnc}
  p-lemma-3 (var x) tâˆˆMF u tâ†’*u = {!  !}  -- p(var) is a nf
  p-lemma-3 (fun aS ts) tâˆˆMF u tâ†’*u = {!  !}  -- p(a) is mf 
  p-lemma-3 (fun bS ts) tâˆˆMF u tâ†’*u = {!  !}  -- p(b) is mf 
  p-lemma-3 {V} (Signature.fun pS (t âˆ· [])) tâˆˆMF u tâ†’*u  
      with p-lemma-1* t u tâ†’*u
  ... | w ,, refl , ptâ†’w with tâˆˆMF w ptâ†’w 
  ... | wâ†’pt = Rfun-cong rules V pS (w âˆ· []) (fun pS (t âˆ· []) âˆ· [] ) Î» { aS â†’ wâ†’pt}
  p-lemma-3 (Signature.fun fS ts) tâˆˆMF u Îµâ‹† = Îµâ‹†
  p-lemma-3 (Signature.fun fS ts) tâˆˆMF u (x ,â‹† tâ†’*u) = {! !}
  p-lemma-3 (fun kS ts) tâˆˆMF u tâ†’*u = {!  !}  -- p(k) is nf

{-
  -- prove t âˆˆ MF â†’ p(t) âˆˆ MF 
  p-lemma-3 : âˆ€ {V} (t : Terms V) â†’ t âˆˆ MF {R = Rnc} â†’ fun pS (t âˆ· []) âˆˆ MF {R = Rnc}
  p-lemma-3 (Signature.var x) tâˆˆMF u tâ†’*u = {!  !} -- âˆˆ NF 
  p-lemma-3 (Signature.fun zero x) tâˆˆMF u tâ†’*u = {! !} -- p(a) is recurrent (hence MF)
  p-lemma-3 (Signature.fun (suc zero) x) tâˆˆMF u tâ†’*u = {! !} -- p(b) âˆˆ MF 
  p-lemma-3 (Signature.fun (suc (suc f)) x) tâˆˆMF u Îµâ‹† = Îµâ‹†
  p-lemma-3 (Signature.fun (suc (suc f)) x) tâˆˆMF u (_,â‹†_ {y = v} (Substitution.Rax (suc (suc (suc zero)) ,, ())) vâ†’*u)
  p-lemma-3 (Signature.fun (suc (suc f)) x) tâˆˆMF u (_,â‹†_ {y = v} (Substitution.Rax (suc (suc (suc (suc ()))) ,, sndâ‚)) vâ†’*u)
  p-lemma-3 (Signature.fun (suc (suc zero)) (x âˆ· [])) tâˆˆMF u (_,â‹†_ {y = v} (Substitution.Rfun (suc (suc zero)) (xâ‚ƒ âˆ· []) zero tâ†’v refl refl) vâ†’*u) = {!tâˆˆMF _ vâ†’*u  !}
  p-lemma-3 (Signature.fun (suc (suc (suc f))) x) tâˆˆMF u (_,â‹†_ {y = v} (Substitution.Rfun (suc (suc zero)) (xâ‚ƒ âˆ· []) zero tâ†’v refl refl) vâ†’*u) = {! !} 
  -- 
  p-lemma-3 t tâˆˆMF u Îµâ‹† = Îµâ‹†
  p-lemma-3 (Signature.var x) tâˆˆMF u (_,â‹†_ {y = v} ptâ†’v vâ†’*u) = {!  !} -- easy, p(x) âˆˆ NF 
  p-lemma-3 (Signature.fun zero x) tâˆˆMF u (_,â‹†_ {y = v} ptâ†’v vâ†’*u) = {! !} -- p(a) -> p(b) âˆˆ MF 
  p-lemma-3 (Signature.fun (suc zero) x) tâˆˆMF u (_,â‹†_ {y = v} ptâ†’v vâ†’*u) = {! !} -- p(b) â†’ p(a) âˆˆ MF 
  -- p-lemma-3 (Signature.fun (suc (suc zero)) x) tâˆˆMF u (_,â‹†_ {y = v} ptâ†’v vâ†’*u) 
  -- p-lemma-3 (Signature.fun (suc (suc zero)) (x âˆ· [])) tâˆˆMF u (_,â‹†_ {y = v} ptâ†’v vâ†’*u) 
  p-lemma-3 (Signature.fun (suc (suc zero)) (x âˆ· [])) tâˆˆMF u (_,â‹†_ {y = v} (Substitution.Rax (suc (suc (suc zero)) ,, ())) vâ†’*u)
  p-lemma-3 (Signature.fun (suc (suc zero)) (x âˆ· [])) tâˆˆMF u (_,â‹†_ {y = v} (Substitution.Rax (suc (suc (suc (suc ()))) ,, sndâ‚)) vâ†’*u)
  -- p-lemma-3 (Signature.fun (suc (suc zero)) (x âˆ· [])) tâˆˆMF u (_,â‹†_ {y = v} (Substitution.Rfun f ts j ptâ†’v xâ‚ xâ‚‚) vâ†’*u)
  p-lemma-3 (Signature.fun (suc (suc zero)) (x âˆ· [])) tâˆˆMF u (_,â‹†_ {y = v} 
    (Substitution.Rfun .pS .(fun (suc (suc zero)) (x âˆ· []) âˆ· []) zero ptâ†’v refl refl) vâ†’*u) 
    = {!   !}
  p-lemma-3 (Signature.fun (suc (suc (suc zero))) x) tâˆˆMF u (_,â‹†_ {y = v} ptâ†’v vâ†’*u) = {! !}
  p-lemma-3 (Signature.fun (suc (suc (suc (suc zero)))) x) tâˆˆMF u (_,â‹†_ {y = v} ptâ†’v vâ†’*u) = {! !}

  RncIsSM : âˆ€ {V} â†’ Rnc {V} isSM 
  RncIsSM (Signature.var x) = {!  !}  -- EASY
  RncIsSM (Signature.fun zero ts) = {! !} -- a âˆˆ NF 
  RncIsSM (Signature.fun (suc zero) ts) = {! !} -- b âˆˆ NF  
  RncIsSM (Signature.fun (suc (suc zero)) (t âˆ· [])) 
    with RncIsSM t 
  ... | MFâŠ†SM m tâˆˆSM = MFâŠ†SM _ (p-lemma-3 t tâˆˆSM)
  ... | SMind u H = SMind _ tâˆˆSM where 
    tâˆˆSM : _ 
    tâˆˆSM y (Substitution.Rax x) = {! x  !} -- p(a) or p(b), hence MF, and SM 
    tâˆˆSM y (Substitution.Rfun (suc (suc zero)) (Signature.var x âˆ· []) zero (Substitution.Rax (suc (suc (suc zero)) ,, ())) refl refl)
    tâˆˆSM y (Substitution.Rfun (suc (suc zero)) (Signature.var x âˆ· []) zero (Substitution.Rax (suc (suc (suc (suc ()))) ,, sndâ‚)) refl refl)
    tâˆˆSM y (Substitution.Rfun (suc (suc zero)) (Signature.fun f x âˆ· []) zero tâ†’y refl refl) = {! H _ tâ†’y   !}
    
  RncIsSM (Signature.fun (suc (suc (suc zero))) ts) = {! !} -- f 
  RncIsSM (Signature.fun (suc (suc (suc (suc zero)))) ts) = {! !} -- k âˆˆ NF 

  a : Terms âŠ¥
  a = fun aS []

  b : Terms âŠ¥
  b = fun bS []

  pa : Terms âŠ¥
  pa = fun pS (a âˆ· [])

  pb : Terms âŠ¥
  pb = fun pS (b âˆ· [])

  k : Terms âŠ¥
  k = fun kS []

  faa : Terms âŠ¥
  faa = fun fS (pa âˆ· pa âˆ· [])

  fba : Terms âŠ¥
  fba = fun fS (pb âˆ· pa âˆ· [])

  p-aâ†’p-b : Rnc pa pb
  p-aâ†’p-b = Rax (zero ,, refl)

  p-bâ†’p-a : Rnc pb pa
  p-bâ†’p-a = Rax ((suc zero) ,, refl)

  faaâ†’k : Rnc faa k
  faaâ†’k = Rax ((suc (suc zero)) ,, refl)

  faaâ†’fba : Rnc faa fba
  faaâ†’fba = Rfun fS (pa âˆ· pa âˆ· []) zero p-aâ†’p-b refl refl
-}
 
